Initial attempt to define state_rel

pancake/time_to_panScript.sml
@@ -9,6 +9,11 @@ val _ = new_theory "time_to_pan"
 val _ = set_grammar_ancestry
         ["pan_common", "mlint", "timeLang", "panLang"];
 
+Definition ohd_def:
+  (ohd [] = (0:num,[])) ∧
+  (ohd (x::xs) = x)
+End
+
 
 Definition ffiBufferAddr_def:
   ffiBufferAddr = 4000w:'a word
@@ -129,18 +134,6 @@ Definition compCondition_def:
                 (compExp clks vname e2)])
 End
 
-(*
-Definition compConditions_def:
-  compConditions clks vname cnds =
-   case cnds of
-   | [] => Const 1w
-   | c::cs => Op And
-                 (compCondition clks vname c ::
-                  compConditions clks vname cs)
-End
-*)
-
-
 Definition compConditions_def:
   (compConditions clks vname [] = Const 1w) ∧
   (compConditions clks vname cs =
@@ -177,9 +170,7 @@ Definition comp_def:
 End
 
 (*
-  («task_ret»,
-  Struct (Struct (empty_consts n) :: MAP Var
-  [«wait_set»; «wake_up_at»; «location»]));
+   case initWakeUp of NONE => Const 0w | SOME n => Const (n2w n));
 *)
 
 Definition task_controller_def:
@@ -188,28 +179,27 @@ Definition task_controller_def:
       [(«loc», Label (toString initLoc));
        («waitSet»,
         case initWakeUp of NONE => Const 1w | _ => Const 0w);  (* not waitSet *)
-       («wakeUpAt»,
-        case initWakeUp of NONE => Const 0w | SOME n => Const (n2w n));
        («isInput», Const 1w); (* not isInput, active low *)
+       («wakeUpAt», Const 0w);
+       («sysTime», Const 0w);
        («ptr1», Const 0w);
        («len1», Const 0w);
        («ptr2», Const ffiBufferAddr);
        («len2», Const ffiBufferSize);
-       («sysTime», Const 0w);
        («taskRet»,
         Struct [Struct (emptyConsts clksLength);
-                Var «waitSet»;
-                Var «wakeUpAt»;
-                Var «loc»])
+                Const 0w; Const 0w; Const 0w])
       ]
       (nested_seq
        [ExtCall «get_time» «ptr1» «len1» «ptr2» «len2»;
         Assign «sysTime» (Load One (Var «ptr2»));
+        Assign «wakeUpAt»
+               (case initWakeUp of
+                | NONE => Const 0w
+                | SOME n => Op Add [Var «sysTime»; Const (n2w n)]);
         Assign «taskRet» (Struct
                           [Struct (mkClks «sysTime» clksLength);
-                           Var «waitSet»;
-                           Var «wakeUpAt»;
-                           Var «loc»]);
+                           Const 0w; Const 0w; Const 0w]);
         While (Const 1w)
               (nested_seq [
                   ExtCall «get_time» «ptr1» «len1» «ptr2» «len2»;
@@ -234,279 +224,24 @@ Definition task_controller_def:
                                (destruct (Field 0 (Var «taskRet»))))
                        (* elapsed time clock variables *)];
                       Assign «waitSet»  (Field 1 (Var «taskRet»));
-                      Assign «wakeUpAt» (Field 2 (Var «taskRet»));
+                      Assign «wakeUpAt»
+                             (Op Add [Var «sysTime»; Field 2 (Var «taskRet»)]);
                       Assign «loc»      (Field 3 (Var «taskRet»))
                     ]
                  ])
         ])
 End
 
-(*
-
-(*
-Definition destruct_def:
-  destruct e xs =
-    MAP (λx. Field x e) xs
-End
-*)
-
-Definition mkStruct_def:
-  mkStruct n vname = Struct (GENLIST (λ_. Var vname) n)
-End
-
-
-
-
-(*
-  FLOOKUP t.locals «clks» = SOME (Struct clkvals)
-  toString dest IN FDOM t.code
-*)
-
-Definition comp_terms_def:
-  (comp_terms fcomp (vname,clks:mlstring list) [] = Skip) ∧
-  (comp_terms fcomp (vname,clks) (t::ts) =
-   let cds = conditions_of t
-   in
-   If (comp_conditions (vname, clks) cds)
-      (fcomp clks t)
-      (comp_terms fcomp (vname,clks) ts))
-End
-
-
-
-
-
-
-
-Definition comp_location_def:
-  comp_location clks (loc, ts) =
-  let n = LENGTH clks in
-    (toString loc,
-     [(«clks», gen_shape n)],
-     comp_terms comp_term («clks»,clks) ts)
-End
-
-
-Definition comp_prog_def:
-  (comp_prog clks [] = []) ∧
-  (comp_prog clks (p::ps) =
-     comp_location clks p :: comp_prog clks ps)
-End
-
-
-Definition comp_def:
-  comp prog =
-    comp_prog (clks_of prog) prog
-End
-
-
-
-(*
-Definition negate_def:
-  negate vname =
-  If  (Cmp Equal (Var vname) (Const 0w))
-      (Assign vname (Const 1w))
-      (Assign vname (Const 0w))
-End
-
-(* calibrate wait time with system time *)
-Definition update_wakeup_time_def:
-  update_wakeup_time (v1,v2) wts =
-    Seq (min_of v1 wts)
-        (Assign v1 (Op Add [Var v1; Var v2]))
-End
-
-(* compile time expressions *)
-Definition comp_exp_def:
-  (comp_exp _ (ELit t) = Const (n2w t)) ∧
-  (comp_exp (vname,clks) (EClock clk) =
-    Field (indice_of clks clk) (Var vname)) ∧
-  (comp_exp clks (ESub e1 e2) =
-   Op Sub [comp_exp clks e1; comp_exp clks e2])
-End
-
-(* compile conditions of time *)
-
-(*
-   TODISC:
-   generating true for [] conditions,
-   to double check with semantics
-*)
-Definition comp_conditions_def:
-  (comp_conditions clks [] = Const 1w) ∧
-  (comp_conditions clks cs = Op And (MAP (comp_condition clks) cs))
-End
-
-
-Definition reset_clocks_def:
-  reset_clocks clks (v1,v2) ns =
-    mk_struct (LENGTH clks) (v1,v2) ns
-End
-
-(*
-Definition destruct_def:
-  destruct e xs =
-    MAP (λx. Field x e) xs
-End
-*)
-
-(*
-  normalisedClocks:
-  Op Sub [Var «clks» - Var «systemTime»]
-  resetClocks:
-  reset_clocks «normalisedClocks» clks_of_term
-  clks_of_wait should be the same
-  and then wait_times should not take systemTime
-*)
-
-
-(*
-   (* reset clks of the term to the system time *)
-   rclocks =  reset_clocks clks («sys_time»,«clks») clks_of_term;
-
-*)
-
-
-Definition comp_term_def:
-  comp_term (clks:mlstring list) (Tm io cnds tclks loc wt) =
-  let clks_of_term = indices_of clks tclks;
-      clks_of_wait = indices_of clks (MAP SND wt);
-
-      (* reset clks of the term to the system time *)
-      rclocks = reset_clocks clks («sys_time»,«clks») clks_of_term;
-
-      (* wait-time should be calculated after resetting the clocks *)
-      clks_of_wait = MAP (λx. Field x rclocks) clks_of_wait;
-      wait_exps = wait_times «sys_time» (MAP FST wt) clks_of_wait;
-
-      return  = Return (
-        Struct
-        [rclocks;
-         Var «wait_set»;
-         Var «wake_up_at»; Label (toString loc)]) in
-    decs [
-        («wait_set»,  case tclks of [] => Const 0w | _ => Const 1w);
-        («wake_up_at», Const (-1w))]
-         (nested_seq
-          [update_wakeup_time («wake_up_at»,«sys_time») wait_exps;
-           case io of
-           | (Input insig)   => return
-           | (Output outsig) =>
-               decs
-               [(«ptr1»,Const 0w);
-                («len1»,Const 0w);
-                («ptr2»,Const ffi_buffer_address);
-                («len2»,Const ffi_buffer_size)
-               ] (Seq
-                  (ExtCall (strlit (toString outsig)) «ptr1» «len1» «ptr2» «len2»)
-                  return)
-          ])
-End
-
-
-
-(*
-  ¬ (is_input ∨ (wait_set ∧ ¬ (sys_time < wake_up_at))) =
-  ¬is_input  ∧ (¬wait_set ∨ (sys_time < wake_up_at))
-*)
-
-
-(* either implement it or return from the task *)
-(*
-Definition not_def:
-  not e =
-    If _ _ _
-End
-*)
-
-(*
-  External functions:
-  get_time, check_input
-*)
-
-
-Definition poll_def:
-  poll =
-    Op And [(*Not*) Var «is_input»;
-            Op Or
-               [(* Not *) Var «wait_set»;
-                Cmp Less (Var «sys_time») (Var «wake_up_at»)]]
-End
-
-
-Definition task_controller_def:
-  task_controller init_loc init_wake_up n =
-     decs
-      [(«location»,Label (toString init_loc));
-       («wait_set»,
-        case init_wake_up of NONE => Const 0w | _ => Const 1w);
-       («wake_up_at»,
-        case init_wake_up of NONE => Const 0w | SOME n => Const (n2w n));
-       («is_input»,Const 0w);
-       («sys_time»,Const 0w);
-       («task_ret»,
-        Struct (Struct (empty_consts n) :: MAP Var
-                [«wait_set»; «wake_up_at»; «location»]));
-       («ptr1»,Const 0w);
-       («len1»,Const 0w);
-       («ptr2»,Const ffi_buffer_address);
-       («len2»,Const ffi_buffer_size)
-      ]
-      (nested_seq
-       [ExtCall «get_time» «ptr1» «len1» «ptr2» «len2»;
-        Assign «sys_time» (Load One (Var «ptr2»));
-        Assign «task_ret»
-               (Struct (mk_clks n «sys_time» :: MAP Var
-                        [«wait_set»; «wake_up_at»; «location»]));
-
-         While (Const 1w)
-               (nested_seq [
-                   negate  «wait_set»;
-                   (* can be optimised, i.e. return the negated wait_set from the function call *)
-                   ExtCall «get_time» «ptr1» «len1» «ptr2» «len2»;
-                   Assign  «sys_time» (Load One (Var «ptr2»));
-                   ExtCall «check_input» «ptr1» «len1» «ptr2» «len2»;
-                   Assign  «is_input» (Load One (Var «ptr2»));
-                   negate  «is_input»;
-                   While (Op And [Var «is_input»; (* Not *)
-                                  Op Or
-                                  [Var «wait_set»; (* Not *)
-                                   Cmp Less (Var «sys_time») (Var «wake_up_at»)]])
-                     (nested_seq [
-                         ExtCall «get_time» «ptr1» «len1» «ptr2» «len2»;
-                         Assign  «sys_time» (Load One (Var «ptr2»));
-                         ExtCall «check_input» «ptr1» «len1» «ptr2» «len2»;
-                         Assign  «is_input» (Load One (Var «ptr2»))]);
-                   nested_seq [
-                       Call (Ret «task_ret» NONE) (Var «location»)
-                       [Var «sys_time»; Field 0 (Var «task_ret»)
-                                        (* elapsed time clock variables *)];
-                       Assign «wait_set»   (Field 1 (Var «task_ret»));
-                       Assign «wake_up_at» (Field 2 (Var «task_ret»));
-                       Assign «location»   (Field 3 (Var «task_ret»))
-                     ]
-                 ])
-        ])
-End
-
-
-Definition ohd_def:
-  (ohd [] = (0:num,[])) ∧
-  (ohd (x::xs) = x)
-End
 
 Definition start_controller_def:
   start_controller (ta_prog:program) =
   let
     prog = FST ta_prog;
-    init_loc = FST (ohd prog);
-    init_wake_up = SND ta_prog;
-    n = number_of_clks prog
+    initLoc = FST (ohd prog);
+    initWakeUp = SND ta_prog;
+    clksLength = nClks prog
   in
-    task_controller init_loc init_wake_up n
+    task_controller initLoc initWakeUp clksLength
 End
 
-*)
-
-*)
 val _ = export_theory();
